examples/layeredeffects/AlgForAll.fst
@@ -10,8 +10,10 @@ module T = FStar.Tactics
 module ID5 = ID5
 open Alg
 
-let post (a:Type) = (a & state) -> Type0
-let st_wp (a:Type) : Type = state -> post a -> Type0
+type rwtree a = Alg.tree a [Read;Write]
+let tbind : #a:_ -> #b:_ -> rwtree a -> (a -> rwtree b) -> rwtree b = fun c f -> Alg.bind _ _ _ _ c f
+
+let st_wp (a:Type) : Type = state -> (a & state -> Type0) -> Type0
 
 unfold
 let return_wp #a x : st_wp a = fun s0 p -> p (x, s0)
@@ -28,7 +30,7 @@ unfold
 let write_wp : state -> st_wp unit = fun s _ p -> p ((), s)
 
 (* Also doable with handlers *)
-let rec interp_as_wp #a (t : repr a [Read;Write]) : st_wp a =
+let rec interp_as_wp #a (t : rwtree a) : st_wp a =
   match t with
   | Return x -> return_wp x
   | Act Read _ k ->
@@ -36,18 +38,8 @@ let rec interp_as_wp #a (t : repr a [Read;Write]) : st_wp a =
   | Act Write s k ->
     bind_wp (write_wp s) (fun (o:unit) -> WF.axiom1 k o; interp_as_wp (k o))
     
-let interp_as_fun #a (t : repr a [Read;Write]) : (state -> a & state) =
+let interp_as_fun #a (t : rwtree a) : (state -> a & state) =
   Alg.interp_rdwr_tree t
-
-// m is a monad.
-val m (a : Type u#a) : Type u#a
-let m a = repr a [Read;Write]
-
-val m_return (#a : Type) : a -> m a
-let m_return x = Return x
-
-val m_bind (#a #b : Type) : m a -> (a -> m b) -> m b
-let m_bind c f = bind _ _ _ _ c f
 
 (* Bug: defining this as a FStar.Preorder.preorder
 causes stupid failures ahead *)
@@ -58,11 +50,7 @@ let equiv #a (w1 w2 : st_wp a) = w1 `stronger` w2 /\ w2 `stronger` w1
 
 let (<<=) = stronger
 
-// a morphism between them, satisfying appropriate laws
-val interp (#a : Type) : m a -> st_wp a
-let interp = interp_as_wp
-
-val interp_ret (#a:Type) (x:a) : Lemma (return_wp x `stronger` interp (m_return x))
+val interp_ret (#a:Type) (x:a) : Lemma (return_wp x `stronger` interp_as_wp (Return x))
 let interp_ret x = ()
 
 let wp_is_monotonic #a (wp : st_wp a) : Type0 =
@@ -73,45 +61,45 @@ let bind_preserves_mon #a #b (wp : st_wp a) (f : a -> st_wp b)
           (ensures (wp_is_monotonic (bind_wp wp f)))
   = ()
 
-let rec interp_monotonic #a (c:m a) : Lemma (wp_is_monotonic (interp c)) =
+let rec interp_monotonic #a (c:rwtree a) : Lemma (wp_is_monotonic (interp_as_wp c)) =
   match c with
   | Return x -> ()
   | Act Read _ k ->
-    let aux (x:state) : Lemma (wp_is_monotonic (interp (k x))) =
+    let aux (x:state) : Lemma (wp_is_monotonic (interp_as_wp (k x))) =
       WF.axiom1 k x;
       interp_monotonic (k x)
     in
     Classical.forall_intro aux;
-    bind_preserves_mon read_wp (fun x -> interp (k x))
+    bind_preserves_mon read_wp (fun x -> interp_as_wp (k x))
   | Act Write s k ->
-    let aux (x:unit) : Lemma (wp_is_monotonic (interp (k x))) =
+    let aux (x:unit) : Lemma (wp_is_monotonic (interp_as_wp (k x))) =
       WF.axiom1 k x;
       interp_monotonic (k x)
     in
     Classical.forall_intro aux;
-    bind_preserves_mon (write_wp s) (fun x -> interp (k x))
+    bind_preserves_mon (write_wp s) (fun x -> interp_as_wp (k x))
 
-let elim_str #a (w1 w2 : st_wp a) (p : post a) (s0:state)
+let elim_str #a (w1 w2 : st_wp a) (p : (a & state -> Type0)) (s0:state)
   : Lemma (requires (w1 <<= w2))
           (ensures w1 s0 p ==> w2 s0 p)
   = ()
 
 (* Takes a while *)
-let rec interp_morph #a #b (c : m a) (f : a -> m b) (p:_) (s0:_)
-  : Lemma (interp c s0 (fun (y, s1) -> interp (f y) s1 p) == interp (m_bind c f) s0 p)
+let rec interp_morph #a #b (c : rwtree a) (f : a -> rwtree b) (p:_) (s0:_)
+  : Lemma (interp_as_wp c s0 (fun (y, s1) -> interp_as_wp (f y) s1 p) == interp_as_wp (tbind c f) s0 p)
   = match c with
     | Return x -> ()
     | Act Read _ k ->
-      let aux (o:state) : Lemma (interp (k o) s0 (fun (y, s1) -> interp (f y) s1 p)
-                                        == interp (m_bind (k o) f) s0 p) =
+      let aux (o:state) : Lemma (interp_as_wp (k o) s0 (fun (y, s1) -> interp_as_wp (f y) s1 p)
+                                        == interp_as_wp (tbind (k o) f) s0 p) =
         WF.axiom1 k o;
         interp_morph (k o) f p s0
       in
       Classical.forall_intro aux
 
     | Act Write s k ->
-      let aux (o:unit) : Lemma (interp (k o) s (fun (y, s1) -> interp (f y) s1 p)
-                                        == interp (m_bind (k o) f) s p) =
+      let aux (o:unit) : Lemma (interp_as_wp (k o) s (fun (y, s1) -> interp_as_wp (f y) s1 p)
+                                        == interp_as_wp (tbind (k o) f) s p) =
         WF.axiom1 k o;
         interp_morph (k o) f p s
       in
@@ -121,38 +109,38 @@ let rec interp_morph #a #b (c : m a) (f : a -> m b) (p:_) (s0:_)
       unreachable ()
 
 val interp_bind (#a #b:Type)
-  (c : m a) (f : a -> m b)
+  (c : rwtree a) (f : a -> rwtree b)
   (w1 : st_wp a) (w2 : a -> st_wp b)
-  : Lemma (requires w1 <<= interp c /\ (forall x. w2 x <<= interp (f x)))
-          (ensures bind_wp w1 w2 `stronger` interp (m_bind c f))
+  : Lemma (requires w1 <<= interp_as_wp c /\ (forall x. w2 x <<= interp_as_wp (f x)))
+          (ensures bind_wp w1 w2 `stronger` interp_as_wp (tbind c f))
 let interp_bind #a #b c f w1 w2 =
-  let aux (p:post b) (s0:state) : Lemma (bind_wp w1 w2 s0 p ==> interp (m_bind c f) s0 p) =
+  let aux (p: (b & state -> Type0)) (s0:state) : Lemma (bind_wp w1 w2 s0 p ==> interp_as_wp (tbind c f) s0 p) =
     calc (==>) {
       bind_wp w1 w2 s0 p;
       ==> {}
       w1 s0 (fun (y, s1) -> w2 y s1 p);
       ==> { (* hyp *)}
-      interp c s0 (fun (y, s1) -> w2 y s1 p);
+      interp_as_wp c s0 (fun (y, s1) -> w2 y s1 p);
       ==> { interp_monotonic c }
-      interp c s0 (fun (y, s1) -> interp (f y) s1 p);
+      interp_as_wp c s0 (fun (y, s1) -> interp_as_wp (f y) s1 p);
       ==> { interp_morph c f p s0 }
-      interp (m_bind c f) s0 p;
+      interp_as_wp (tbind c f) s0 p;
     }
   in
   Classical.forall_intro_2 aux
 
-let repr (a : Type) (w: st_wp a) = c:(m a){w `stronger` interp c}
+let repr (a : Type) (w: st_wp a) = c:(rwtree a){w `stronger` interp_as_wp c}
 
 let return (a:Type) (x:a) : repr a (return_wp x) =
   interp_ret x;
-  m_return x
+  Return x
 
 let bind (a : Type) (b : Type)
   (wp_v : st_wp a) (wp_f: a -> st_wp b)
   (v : repr a wp_v) (f : (x:a -> repr b (wp_f x)))
   : repr b (bind_wp wp_v wp_f) =
   interp_bind v f wp_v wp_f;
-  m_bind v f
+  tbind v f
 
 let subcomp (a:Type) (w1 w2: st_wp a)
   (f : repr a w1)
@@ -168,7 +156,7 @@ total
 reifiable
 reflectable
 layered_effect {
-  DM4A : a:Type -> st_wp a -> Effect
+  AlgWP : a:Type -> st_wp a -> Effect
   with repr         = repr;
        return       = return;
        bind         = bind;
@@ -176,49 +164,37 @@ layered_effect {
        if_then_else = if_then_else
 }
 
-let _get : repr state read_wp =
-  let c0 : Alg.repr state [Read;Write] = Alg._get in
-  let w = interp_as_wp c0 in
-  assert_norm (read_wp `stronger` w);
-  c0
+let get () : AlgWP state read_wp =
+  AlgWP?.reflect (Act Read () Return)
 
-let get () : DM4A state read_wp =
-  DM4A?.reflect _get
-
-let _put (s:state) : repr unit (write_wp s) =
-  let c0 : Alg.repr unit [Read;Write] = Alg._put s in
-  let w = interp_as_wp c0 in
-  assert_norm (write_wp s `stronger` w);
-  c0
-
-let put (s:state) : DM4A unit (write_wp s) =
-  DM4A?.reflect (_put s)
+let put (s:state) : AlgWP unit (write_wp s) =
+  AlgWP?.reflect (Act Write s Return)
 
 unfold
 let lift_pure_wp (#a:Type) (wp : pure_wp a) : st_wp a =
   fun s0 p -> wp (fun x -> p (x, s0))
 
-let lift_pure_dm4a (a:Type) wp (f:(eqtype_as_type unit -> PURE a wp))
+let lift_pure_algwp (a:Type) wp (f:(eqtype_as_type unit -> PURE a wp))
   : Pure (repr a (lift_pure_wp wp)) // can't call f() here, so lift its wp instead
          (requires (wp (fun _ -> True)))
          (ensures (fun _ -> True))
   =
     let v : a = elim_pure f (fun _ -> True) in
-    FStar.Monotonic.Pure.wp_monotonic_pure ();
+    FStar.Monotonic.Pure.wp_monotonic_pure (); // need this lemma
     assert (forall p. wp p ==> p v); // this is key fact needed for the proof
     assert_norm (stronger (lift_pure_wp wp) (return_wp v));
     Return v
 
-sub_effect PURE ~> DM4A = lift_pure_dm4a
+sub_effect PURE ~> AlgWP = lift_pure_algwp
 
-let addx (x:int) : DM4A unit (fun s0 p -> p ((), (s0+x))) =
+let addx (x:int) : AlgWP unit (fun s0 p -> p ((), (s0+x))) =
   let y = get () in
   put (x+y)
 
 (* GM: this used to require a call to T.norm [delta] when I had curry/uncurry going on.
 I now realize they were not marked unfold, but that is pretty tricky... we should try
 to find some general solution for these things. *)
-let add_via_state (x y : int) : DM4A int (fun s0 p -> p ((x+y), s0)) =
+let add_via_state (x y : int) : AlgWP int (fun s0 p -> p ((x+y), s0)) =
   let o = get () in
   put x;
   addx y;
@@ -229,14 +205,14 @@ let add_via_state (x y : int) : DM4A int (fun s0 p -> p ((x+y), s0)) =
 
 // Why does this admit fail? Only with the 'rec'...
 //
-//let rec interp_sem #a #wp (t : repr a wp) (s0:state)
-//  : PURE (a & state) (fun p -> wp s0 (curry p))
-//  = admit ()
+// let rec interp_sem #a #wp (t : repr a wp) (s0:state)
+//   : PURE (a & state) (fun p -> wp s0 p)
+//   = admit ()
 //
 // literally zero difference in the VC a tactic sees. Also, seems only
 // for the builtin Pure???
 
-let rec interp_sem #a (t : m a) (s0:state)
+let rec interp_sem #a (t : rwtree a) (s0:state)
   : ID5.ID (a & state) (interp_as_wp t s0)
   = match t with
     | Return x -> (x, s0)
@@ -247,7 +223,7 @@ let rec interp_sem #a (t : m a) (s0:state)
       WF.axiom1 k ();
       interp_sem (k ()) i
     
-let soundness #a #wp (t : unit -> DM4A a wp)
+let soundness #a #wp (t : unit -> AlgWP a wp)
   : Tot (s0:state -> ID5.ID (a & state) (wp s0))
   = let c = reify (t ()) in
-    interp_sem #_ c
+    interp_sem c
